theories/persistent/PLAN.md
@@ -7,16 +7,21 @@
   ALEX: perhaps, leaving it for now.
 
 - extend `undo` with a correct update of the ρg in addition to the ρv.
+  ALEX:DONE
 
 - The map-model M returns a (ref_loc -> val) mapping for each
   node. Complement it with a new MG which returns
   a (ref_loc -> generation) mapping for each node – or maybe extend
   M to return both, if it does not induce too much proof churn.
+  ALEX: I chose the second option, easier and DONE.
 
   Invariants:
-  - something like correct-path-diff, for generations in addition to values
+  - something like correct-path-diff, for generations in addition to
+    values
+  ALEX: DONE
   - MG(orig) is the constant-0 function
   - MG(root) is the current ρg
+  ALEX: DONE
 
   This does not help reason about record elision, but it is the part
   that specifies the correct generation to store in diff nodes. I hope
@@ -25,8 +30,8 @@
 
 - Define a function/relation that computes the "last write to r": walk
   up the path from orig to root in the current graph (walking up: from
-  root to orig). If n is the first node along the way to record
-  a change for r, we have G(n) = ρg(r).
+  root to orig).
+  ALEX: DONE: see `lwt`.
 
   Note: if we can define this in term of the current graph, maybe we
   did not need to introduce the history graph after all? To be
@@ -35,6 +40,8 @@
 - Invariant: there is a correspondence between the current ρg and the
   generation of the last write of each reference. If the node `n` is
   the last write of `r`, they have the same generation: G(n) = ρg(r).
+  ALEX: ALMOST DONE (see `history_inv`), except for restore.
+  Should be ok.
 
 - Lemma: if `n` is the last write node for `r`, and ρg(r) is equal to
   the generation of the store, then none of the transitive children of
